finished with frontend files up to Cexec

cfrontend/Cexec.v
@@ -451,6 +451,12 @@ Definition do_ef_malloc
   | _ => None
   end.
 
+(*SACC:*)
+Definition dec_not {A B}: {A}+{B} -> {B}+{A}.
+Proof.
+  intros [a|a];[right|left]; auto.
+Defined.
+
 Definition do_ef_free
        (w: world) (vargs: list val) (m: mem) : option (world * trace * val * mem) :=
   match vargs with
@@ -458,6 +464,7 @@ Definition do_ef_free
       do vsz <- Mem.load Mptr m b (Ptrofs.unsigned lo - size_chunk Mptr);
       do sz <- do_alloc_size vsz;
       check (zlt 0 (Ptrofs.unsigned sz));
+(*SACC:*)check (dec_not (in_stack_dec (Mem.stack m) b));
       do m' <- Mem.free m b (Ptrofs.unsigned lo - size_chunk Mptr) (Ptrofs.unsigned lo + Ptrofs.unsigned sz);
       Some(w, E0, Vundef, m')
   | _ => None
@@ -510,7 +517,7 @@ Definition do_external (ef: external_function):
   | EF_vload chunk => do_ef_volatile_load chunk
   | EF_vstore chunk => do_ef_volatile_store chunk
   | EF_malloc => do_ef_malloc
-  | EF_free => do_ef_free
+(*SACC: commented this*)(*  | EF_free => do_ef_free*)
   | EF_memcpy sz al => do_ef_memcpy sz al
   | EF_annot text targs => do_ef_annot text targs
   | EF_annot_val text targ => do_ef_annot_val text targ
@@ -549,8 +556,9 @@ Proof with try congruence.
   destruct (Mem.alloc m (- size_chunk Mptr) (Ptrofs.unsigned i)) as [m1 b] eqn:?. mydestr.
   split. apply SIZE in Heqo. subst v. econstructor; eauto. constructor.
 (* EF_free *)
-  unfold do_ef_free. destruct vargs... destruct v... destruct vargs...
-  mydestr. split. apply SIZE in Heqo0. econstructor; eauto. congruence. omega. constructor.
+(*SACC: commented this*)
+(*  unfold do_ef_free. destruct vargs... destruct v... destruct vargs...
+  mydestr. split. apply SIZE in Heqo0. econstructor; eauto. congruence. omega. constructor.*)
 (* EF_memcpy *)
   unfold do_ef_memcpy. destruct vargs... destruct v... destruct vargs...
   destruct v... destruct vargs... mydestr. 
@@ -596,8 +604,9 @@ Proof.
   inv H; unfold do_ef_malloc.
   inv H0. erewrite SIZE by eauto. rewrite H1, H2. auto.
 (* EF_free *)
-  inv H; unfold do_ef_free.
-  inv H0. rewrite H1. erewrite SIZE by eauto. rewrite zlt_true. rewrite H3. auto. omega.
+(*SACC: commented this*)
+(*  inv H; unfold do_ef_free.
+  inv H0. rewrite H1. erewrite SIZE by eauto. rewrite zlt_true. rewrite H3. auto. omega.*)
 (* EF_memcpy *)
   inv H; unfold do_ef_memcpy.
   inv H0. rewrite Decidable_complete. rewrite H7; rewrite H8; auto.
@@ -619,7 +628,7 @@ Qed.
 Inductive reduction: Type :=
   | Lred (rule: string) (l': expr) (m': mem)
   | Rred (rule: string) (r': expr) (m': mem) (t: trace)
-  | Callred (rule: string) (fd: fundef) (args: list val) (tyres: type) (m': mem)
+  | Callred (rule: string) (fd: fundef) (args: list val) (tyres: type) (m': mem) (*SACC:*)(fid : ident)
   | Stuckred.
 
 Section EXPRS.
@@ -848,10 +857,11 @@ Fixpoint step_expr (k: kind) (a: expr) (m: mem): reducts expr :=
       | Some(vf, tyf), Some vtl =>
           match classify_fun tyf with
           | fun_case_f tyargs tyres cconv =>
+     (*SACC:*)do fid <- Globalenvs.invert_pointer ge vf;
               do fd <- Genv.find_funct ge vf;
               do vargs <- sem_cast_arguments vtl tyargs m;
               check type_eq (type_of_fundef fd) (Tfunction tyargs tyres cconv);
-              topred (Callred "red_call" fd vargs ty m)
+              topred (Callred "red_call" fd vargs ty ((*SACC:*)Mem.push_new_stage m) (*SACC:*)fid)
           | _ => stuck
           end
       | _, _ =>
@@ -862,9 +872,11 @@ Fixpoint step_expr (k: kind) (a: expr) (m: mem): reducts expr :=
       match is_val_list rargs with
       | Some vtl =>
           do vargs <- sem_cast_arguments vtl tyargs m;
-          match do_external ef w vargs m with
+          match do_external ef w vargs ((*SACC:*)Mem.push_new_stage m) with
           | None => stuck
-          | Some(w',t,v,m') => topred (Rred "red_builtin" (Eval v ty) m' t)
+          | Some(w',t,v,m') => 
+     (*SACC:*)do m'' <- Mem.unrecord_stack_block m';
+              topred (Rred "red_builtin" (Eval v ty) ((*SACC:*)m'') t)
           end
       | _ =>
           incontext (fun x => Ebuiltin ef tyargs x ty) (step_exprlist rargs m)
@@ -896,8 +908,8 @@ Inductive imm_safe_t: kind -> expr -> mem -> Prop :=
       rred ge r m t r' m' -> possible_trace w t w' ->
       context RV to C ->
       imm_safe_t to (C r) m
-  | imm_safe_t_callred: forall to C r m fd args ty,
-      callred ge r m fd args ty ->
+  | imm_safe_t_callred: forall to C r m fd args ty (*SACC:*)fid,
+      callred ge r m fd args ty (*SACC:*)fid ->
       context RV to C ->
       imm_safe_t to (C r) m.
 
@@ -965,16 +977,18 @@ Definition invert_expr_prop (a: expr) (m: mem) : Prop :=
       exists v, sem_cast v1 ty1 tycast m = Some v
   | Ecall (Eval vf tyf) rargs ty =>
       exprlist_all_values rargs ->
-      exists tyargs tyres cconv fd vl,
+      exists tyargs tyres cconv fd vl fid,
+  (*SACC:*)is_function_ident ge vf fid /\
          classify_fun tyf = fun_case_f tyargs tyres cconv
       /\ Genv.find_funct ge vf = Some fd
       /\ cast_arguments m rargs tyargs vl
       /\ type_of_fundef fd = Tfunction tyargs tyres cconv
   | Ebuiltin ef tyargs rargs ty =>
       exprlist_all_values rargs ->
-      exists vargs t vres m' w',
+      exists vargs t vres m' (*SACC:*)m'' w',
          cast_arguments m rargs tyargs vargs
-      /\ external_call ef ge vargs m t vres m'
+      /\ external_call ef ge vargs (Mem.push_new_stage m) t vres m'
+  (*SACC*)/\ Mem.unrecord_stack_block m' = Some m''
       /\ possible_trace w t w'
   | _ => True
   end.
@@ -1005,16 +1019,16 @@ Proof.
   exists t; exists v1; exists w'; auto.
   exists t; exists v1; exists w'; auto.
   exists v; auto.
-  intros; exists vargs; exists t; exists vres; exists m'; exists w'; auto.
+  intros; exists vargs; exists t; exists vres; exists m', m''; exists w'; auto.
 Qed.
 
 Lemma callred_invert:
-  forall r fd args ty m,
-  callred ge r m fd args ty ->
+  forall r fd args ty m (*SACC:*)fid,
+  callred ge r m fd args ty (*SACC:*)fid ->
   invert_expr_prop r m.
 Proof.
   intros. inv H. simpl.
-  intros. exists tyargs, tyres, cconv, fd, args; auto.
+  intros. exists tyargs, tyres, cconv, fd, args, fid; auto.
 Qed.
 
 Scheme context_ind2 := Minimality for context Sort Prop
@@ -1106,7 +1120,7 @@ Definition reduction_ok (k: kind) (a: expr) (m: mem) (rd: reduction) : Prop :=
   match k, rd with
   | LV, Lred _ l' m' => lred ge e a m l' m'
   | RV, Rred _ r' m' t => rred ge a m t r' m' /\ exists w', possible_trace w t w'
-  | RV, Callred _ fd args tyres m' => callred ge a m fd args tyres /\ m' = m
+  | RV, Callred _ fd args tyres m' (*SACC:*)fid => callred ge a m fd args tyres (*SACC:*)fid /\ (*SACC:*)m' = Mem.push_new_stage m
   | LV, Stuckred => ~imm_safe_t k a m
   | RV, Stuckred => ~imm_safe_t k a m
   | _, _ => False
@@ -1459,15 +1473,21 @@ Proof with (try (apply not_invert_ok; simpl; intro; myinv; intuition congruence;
   rewrite (is_val_inv _ _ _ Heqo). exploit is_val_list_all_values; eauto. intros ALLVAL.
   (* top *)
   destruct (classify_fun tyf) as [tyargs tyres cconv|] eqn:?...
+  destruct (invert_pointer ge vf) eqn:?...
   destruct (Genv.find_funct ge vf) as [fd|] eqn:?...
   destruct (sem_cast_arguments vtl tyargs m) as [vargs|] eqn:?...
   destruct (type_eq (type_of_fundef fd) (Tfunction tyargs tyres cconv))...
   apply topred_ok; auto. red. split; auto. eapply red_call; eauto.
+  apply is_function_ident_invert_pointer_equiv; eauto.
   eapply sem_cast_arguments_sound; eauto.
   apply not_invert_ok; simpl; intros; myinv. specialize (H ALLVAL). myinv. congruence.
   apply not_invert_ok; simpl; intros; myinv. specialize (H ALLVAL). myinv.
   exploit sem_cast_arguments_complete; eauto. intros [vtl' [P Q]]. congruence.
   apply not_invert_ok; simpl; intros; myinv. specialize (H ALLVAL). myinv. congruence.
+  apply not_invert_ok; simpl; intros; myinv. specialize (H ALLVAL). myinv.
+  destruct vf; simpl in *; try congruence.
+  destruct H as (bb & oo & ? & ?). inv H.
+  apply Genv.find_invert_symbol in H4; congruence.
   apply not_invert_ok; simpl; intros; myinv. specialize (H ALLVAL). myinv. congruence.
   (* depth *)
   eapply incontext2_list_ok; eauto.
@@ -1477,11 +1497,14 @@ Proof with (try (apply not_invert_ok; simpl; intro; myinv; intuition congruence;
   exploit is_val_list_all_values; eauto. intros ALLVAL.
   (* top *)
   destruct (sem_cast_arguments vtl tyargs m) as [vargs|] eqn:?...
-  destruct (do_external ef w vargs m) as [[[[? ?] v] m'] | ] eqn:?...
+  destruct (do_external ef w vargs (Mem.push_new_stage m)) as [[[[? ?] v] m'] | ] eqn:?...
   exploit do_ef_external_sound; eauto. intros [EC PT].
+  destruct (Mem.unrecord_stack_block m') eqn:?...
   apply topred_ok; auto. red. split; auto. eapply red_builtin; eauto.
   eapply sem_cast_arguments_sound; eauto.
   exists w0; auto.
+  edestruct (Mem.unrecord_stack_block_succeeds) as (m2' & USB & EQSTK); [|rewrite USB in Heqo2; congruence].
+  repeat rewrite_stack_blocks. reflexivity.
   apply not_invert_ok; simpl; intros; myinv. specialize (H ALLVAL). myinv.
   assert (x = vargs).
     exploit sem_cast_arguments_complete; eauto. intros [vtl' [A B]]. congruence.
@@ -1584,17 +1607,20 @@ Proof.
 (* builtin *)
   exploit sem_cast_arguments_complete; eauto. intros [vtl [A B]].
   exploit do_ef_external_complete; eauto. intros C.
-  rewrite A. rewrite B. rewrite C. econstructor; eauto.
+  rewrite A. rewrite B. rewrite C, H1. econstructor; eauto.
 Qed.
 
 Lemma callred_topred:
-  forall a fd args ty m,
-  callred ge a m fd args ty ->
-  exists rule, step_expr RV a m = topred (Callred rule fd args ty m).
+  forall a fd args ty (*SACC:*)fid m,
+  callred ge a m fd args ty (*SACC:*)fid ->
+  exists rule, step_expr RV a m = topred (Callred rule fd args ty ((*SACC:*)Mem.push_new_stage m) (*SACC:*)fid).
 Proof.
   induction 1; simpl.
-  rewrite H2. exploit sem_cast_arguments_complete; eauto. intros [vtl [A B]].
-  rewrite A; rewrite H; rewrite B; rewrite H1; rewrite dec_eq_true. econstructor; eauto.
+  rewrite H3. exploit sem_cast_arguments_complete; eauto. intros [vtl [A B]].
+  destruct H as (bb & oo & IFI & IFI'). subst. simpl in *.
+  rewrite A; rewrite H0; rewrite B; rewrite H2.
+  erewrite Genv.find_invert_symbol; eauto.
+  rewrite dec_eq_true. econstructor; eauto. 
 Qed.
 
 Definition reducts_incl {A B: Type} (C: A -> B) (res1: reducts A) (res2: reducts B) : Prop :=
@@ -1819,14 +1845,17 @@ Qed.
 (** A state can "crash the world" if it can make an observable transition
   whose trace is not accepted by the external world. *)
 
+(*SACC:*)
+Variable fn_stack_requirements : ident -> Z.
+
 Definition can_crash_world (w: world) (S: state) : Prop :=
-  exists t, exists S', Csem.step ge S t S' /\ forall w', ~possible_trace w t w'.
+  exists t, exists S', Csem.step ((*SACC:*)fn_stack_requirements) ge S t S' /\ forall w', ~possible_trace w t w'.
 
 Theorem not_imm_safe_t:
   forall K C a m f k,
   context K RV C ->
   ~imm_safe_t K a m ->
-  Csem.step ge (ExprState f (C a) k e m) E0 Stuckstate \/ can_crash_world w (ExprState f (C a) k e m).
+  Csem.step ((*SACC:*)fn_stack_requirements) ge (ExprState f (C a) k e m) E0 Stuckstate \/ can_crash_world w (ExprState f (C a) k e m).
 Proof.
   intros. destruct (classic (imm_safe ge e K a m)).
   exploit imm_safe_imm_safe_t; eauto.
@@ -1866,6 +1895,231 @@ Proof.
   rewrite H; rewrite IHalloc_variables; auto.
 Qed.
 
+(*======================================SACC======================================*)
+(*
+Lemma alloc_variables_perm_1:
+  forall (ge: genv) e1 m1 vars e2 m2,
+    alloc_variables ge e1 m1 vars e2 m2 ->
+    forall b o k p,
+      Mem.perm m1 b o k p ->
+      Mem.perm m2 b o k p.
+Proof.
+  induction 1; simpl; intros b o k p P. auto.
+  eapply IHalloc_variables.
+  eapply Mem.perm_alloc_1; eauto.
+Qed.
+
+
+Lemma alloc_variables_perm_2:
+  forall (ge: genv) e1 m1 vars e2 m2,
+    alloc_variables ge e1 m1 vars e2 m2 ->
+    forall b o k p,
+      Mem.valid_block m1 b ->
+      Mem.perm m2 b o k p ->
+      Mem.perm m1 b o k p.
+Proof.
+  induction 1; simpl; intros b o k p V P. auto.
+  eapply IHalloc_variables in P.
+  eapply Mem.perm_alloc_inv in P; eauto.
+  destr_in P. subst. eapply Mem.fresh_block_alloc in V; eauto. easy.
+  eapply Mem.valid_block_alloc; eauto.
+Qed.
+
+Lemma alloc_variables_not_in_vars:
+  forall ge e1 m1 vars e2 m2,
+    alloc_variables ge e1 m1 vars e2 m2 ->
+    forall id,
+      ~ In id (map fst vars) ->
+      e1 ! id = e2 ! id.
+Proof.
+  induction 1; simpl; intros id0 NIN. auto.
+  destruct (peq id0 id). subst. intuition congruence.
+  erewrite <- IHalloc_variables; auto. rewrite PTree.gso. auto. auto.
+Qed.
+
+Lemma alloc_variables_perm:
+  forall ge e1 m1 vars e2 m2,
+    alloc_variables ge e1 m1 vars e2 m2 ->
+    list_norepet (map fst vars) ->
+    forall id b ty o k p,
+      e1 ! id = None ->
+      e2 ! id = Some (b,ty) ->
+      Mem.perm m2 b o k p ->
+      0 <= o < sizeof ge ty.
+Proof.
+  induction 1; simpl; intros LNR id0 b ty0 o k p E1 E2.
+  congruence.
+  inv LNR.
+  destruct (peq id id0). subst.
+  - erewrite <- alloc_variables_not_in_vars in E2; eauto.
+    rewrite PTree.gss in E2; inv E2.
+    intro P.
+    eapply alloc_variables_perm_2 in P. 2: eauto.
+    eapply Mem.perm_alloc_3; eauto.
+    eapply Mem.valid_new_block; eauto.
+  - eapply IHalloc_variables; eauto. rewrite PTree.gso; auto.
+Qed.
+
+Lemma do_alloc_variables_perms:
+  forall  m1 l e2 m2,
+    alloc_variables ge empty_env m1 l e2 m2 ->
+    list_norepet (map fst l) ->
+    Forall
+      (fun b : block * frame_info =>
+         forall (o : Z) (k : perm_kind) (p : permission),
+           Mem.perm m2 (fst b) o k p -> 0 <= o < frame_size (snd b)) (blocks_with_info ge e2).
+Proof.
+  intros m1 l e2 m2 AV LNR.
+  rewrite ! Forall_forall.
+  intros (b & fi) IN o k p PERM.
+  simpl in *.
+  unfold blocks_with_info, blocks_of_env in IN.
+  rewrite !map_map, in_map_iff in IN.
+  destruct IN as ((id & (bb & ty)) & EQ & IN). inv EQ. simpl.
+  exploit alloc_variables_perm. eauto. auto. apply PTree.gempty.
+  eapply PTree.elements_complete. eauto. eauto.
+  intros; rewrite Z.max_r; omega.
+Qed.
+*)
+Lemma list_norepet_map:
+  forall {A B} (f: A -> B) (l: list A) (lnr: list_norepet (map f l)),
+    list_norepet l.
+Proof.
+  induction l; simpl; intros; inv lnr; constructor; eauto. intro NIN; apply H1, in_map; auto.
+Qed.
+
+Lemma do_alloc_variables_norepet:
+  forall
+    v (lnr: list_norepet (map fst v)) e m e' m'
+    (DAV: do_alloc_variables e m v = (e', m'))
+    (REC: forall i1 i2 (diff: i1 <> i2) b1 b2 t1 t2
+              (EQ1: e ! i1 = Some (b1,t1))
+              (EQ2: e ! i2 = Some (b2,t2)),
+          b1 <> b2)
+      (VALID: forall i b t, e ! i = Some (b, t) -> Plt b (Mem.nextblock m))
+      i1 i2 (diff: i1 <> i2) b1 b2 t1 t2
+      (EQ1: e' ! i1 = Some (b1,t1))
+      (EQ2: e' ! i2 = Some (b2,t2)),
+      b1 <> b2.
+Proof.
+  induction v; simpl; intros; eauto.
+  inv DAV; eauto.
+  repeat destr_in DAV.
+  inv lnr. trim IHv. auto.
+  eapply IHv; eauto.
+  {
+    intros i0 i3 diff0 b0 b3 t0 t3.
+    rewrite ! PTree.gsspec.
+    destr. inversion 1; subst.
+    apply Mem.alloc_result in Heqp0. subst.
+    destr. intro EQ3. apply VALID in EQ3. intro; subst. xomega.
+    intro EQ0. 
+    destr. intro EQ3. inv EQ3.
+    apply VALID in EQ0. apply Mem.alloc_result in Heqp0. intro; subst. xomega.
+    intros. eauto.
+  }
+  {
+    intros. exploit Mem.nextblock_alloc. eauto. intro NB; rewrite NB.
+    rewrite PTree.gsspec in H. destr_in H. inv H.
+    exploit Mem.alloc_result. eauto. intro; subst; xomega.
+    eapply VALID in H. xomega.
+  }
+Qed.
+
+Program Definition alloc_variables_record f m sz : option (env * mem) :=
+  check (list_norepet_dec ident_eq (var_names (fn_params f) ++ var_names (fn_vars f)));
+    let '(e,m1) := do_alloc_variables empty_env m (f.(fn_params) ++ f.(fn_vars)) in
+    do m1 <- Mem.record_stack_blocks m1 (Build_frame_adt (blocks_with_info ge e) (Z.max 0 sz) _ _);
+      Some (e,m1).
+Next Obligation.
+  unfold blocks_with_info. unfold blocks_of_env.
+  rewrite ! map_map.
+  apply list_map_norepet.
+  eapply list_norepet_map.
+  apply PTree.elements_keys_norepet.
+  simpl; intros. unfold block_of_binding. repeat destr.
+  subst. repeat destr_in Heqp. repeat destr_in Heqp1. simpl. intro; subst.
+  apply PTree.elements_complete in H0.
+  apply PTree.elements_complete in H1.
+  destruct (peq i i0). subst. apply H2. congruence.
+  exploit do_alloc_variables_norepet. 2: eauto. rewrite map_app. apply H. setoid_rewrite PTree.gempty; congruence.
+  setoid_rewrite PTree.gempty; congruence. apply n. eauto. eauto. auto. auto.
+Qed.
+Next Obligation.
+  apply Z.le_max_l.
+Qed.
+(*
+Lemma destr_dep_match:
+  forall {A B: Type} (a: option A) (x: B)
+    (T: forall x (pf: Some x = a), B)
+    (MATCH: match a as ano return (ano = a -> option B) with
+            | Some m1 => fun Heq: Some m1 = a => Some (T _ Heq)
+            | None => fun Heq => None
+            end eq_refl = Some x) ,
+  forall P: B -> Prop,
+    (forall m (pf: Some m = a) x, T m pf = x -> P x) ->
+    P x.
+Proof.
+  intros. destr_in MATCH. subst. inv MATCH. eapply H. eauto.
+Qed.
+
+Lemma constr_match:
+  forall {A B: Type} (a: option A)
+    x (EQ: a = Some x)
+    (T: forall x (pf: Some x = a), option B)
+    X
+    (EQ: T _ (eq_sym EQ) = Some X),
+    (match a as ano return (ano = a -> option B) with
+       Some m1 =>
+       fun Heq : Some m1 = a => T m1 Heq
+     | None => fun _ => None
+     end) eq_refl = Some X.
+Proof.
+  intros. subst. simpl in *.  auto. 
+Qed.
+*)
+
+Lemma destr_dep_let:
+  forall {A1 A2 B: Type} (a: A1*A2) (bres: B) (T: forall m b (p: (m,b) = a), option B),
+    (let (m,b) as ano return (ano = a -> option B) := a in
+     fun Heq : (m,b) = a => T _ _ Heq) eq_refl = Some bres ->
+    forall (P: B -> Prop),
+      (forall m b (pf: (m, b) = a) x, T _ _ pf = Some x -> P x) ->
+      P bres.
+Proof.
+  intros. destruct a. apply H0 in H; auto.
+Qed.
+
+Lemma alloc_variables_record_spec:
+  forall f m sz e m',
+    alloc_variables_record f m sz = Some (e,m') ->
+    list_norepet (var_names (fn_params f) ++ var_names (fn_vars f)) /\
+    exists m1 fa,
+      alloc_variables ge empty_env m (f.(fn_params) ++ f.(fn_vars)) e m1 /\
+      frame_adt_blocks fa = blocks_with_info ge e /\
+      frame_adt_size fa = Z.max 0 sz /\
+      Mem.record_stack_blocks m1 fa = Some m'.
+Proof.
+  unfold alloc_variables_record.
+  intros f m sz e m' AV.
+  destr_in AV.
+  split; auto. 
+  change ((fun em =>
+            exists (m1 : mem) (fa : frame_adt),
+              alloc_variables ge empty_env m (fn_params f ++ fn_vars f) (fst em) m1 /\
+              frame_adt_blocks fa = blocks_with_info ge (fst em) /\
+              frame_adt_size fa = Z.max 0 sz /\ Mem.record_stack_blocks m1 fa = Some (snd em)) (e,m')).
+  eapply (destr_dep_let (B:=env*mem) (do_alloc_variables empty_env m (fn_params f ++ fn_vars f))).
+  apply AV. clear AV.
+  intros.
+  simpl in H. destr_in H. inv H.
+  exploit do_alloc_variables_sound. rewrite <- pf. simpl.
+  intro AV. rewrite <- Heqo.
+  eexists b, _; repeat split; eauto.
+Qed.
+
+(*======================================CCAS======================================*)
+
 Function sem_bind_parameters (w: world) (e: env) (m: mem) (l: list (ident * type)) (lv: list val)
                           {struct l} : option mem :=
   match l, lv  with
@@ -1903,11 +2157,14 @@ Qed.
 
 Inductive transition : Type := TR (rule: string) (t: trace) (S': state).
 
+(*SACC:*)
+Variable fn_stack_requirements: ident -> Z.
+
 Definition expr_final_state (f: function) (k: cont) (e: env) (C_rd: (expr -> expr) * reduction) :=
   match snd C_rd with
   | Lred rule a m => TR rule E0 (ExprState f (fst C_rd a) k e m)
   | Rred rule a m t => TR rule t (ExprState f (fst C_rd a) k e m)
-  | Callred rule fd vargs ty m => TR rule E0 (Callstate fd vargs (Kcall f e (fst C_rd) ty k) m)
+  | Callred rule fd vargs ty m (*SACC:*)fid => TR rule E0 (Callstate fd vargs (Kcall f e (fst C_rd) ty k) m ((*SACC:*)fn_stack_requirements fid))
   | Stuckred => TR "step_stuck" E0 Stuckstate
   end.
 
@@ -2018,19 +2275,22 @@ Definition do_step (w: world) (s: state) : list transition :=
       | Some(s', k') => ret "step_goto" (State f s' k' e m)
       | None => nil
       end
-
-  | Callstate (Internal f) vargs k m =>
-      check (list_norepet_dec ident_eq (var_names (fn_params f) ++ var_names (fn_vars f)));
-      let (e,m1) := do_alloc_variables empty_env m (f.(fn_params) ++ f.(fn_vars)) in
+  (*SACC:*)
+  | Callstate (Internal f) vargs k m (*SACC:*)sz =>
+    match alloc_variables_record f m (Z.max 0 sz) with
+      Some (e,m1) =>
       do m2 <- sem_bind_parameters w e m1 f.(fn_params) vargs;
-      ret "step_internal_function" (State f f.(fn_body) k e m2)
-  | Callstate (External ef _ _ _) vargs k m =>
+        ret "step_internal_function" (State f f.(fn_body) k e m2)
+    | None => nil
+    end
+  | Callstate (External ef _ _ _) vargs k m  (*SACC:*) _ =>
       match do_external ef w vargs m with
       | None => nil
       | Some(w',t,v,m') => TR "step_external_function" t (Returnstate v k m') :: nil
       end
 
   | Returnstate v (Kcall f e C ty k) m =>
+  (*SACC:*)do m <- Mem.unrecord_stack_block m ;
       ret "step_returnstate" (ExprState f (C (Eval v ty)) k e m)
 
   | _ => nil
@@ -2057,7 +2317,7 @@ Hint Extern 3 => exact I.
 Theorem do_step_sound:
   forall w S rule t S',
   In (TR rule t S') (do_step w S) ->
-  Csem.step ge S t S' \/ (t = E0 /\ S' = Stuckstate /\ can_crash_world w S).
+  Csem.step ((*SACC:*)fn_stack_requirements) ge S t S' \/ (t = E0 /\ S' = Stuckstate /\ can_crash_world ((*SACC:*)fn_stack_requirements) w S).
 Proof with try (left; right; econstructor; eauto; fail).
   intros until S'. destruct S; simpl.
 (* State *)
@@ -2094,10 +2354,12 @@ Proof with try (left; right; econstructor; eauto; fail).
 (* callstate *)
   destruct fd; myinv.
   (* internal *)
-  destruct (do_alloc_variables empty_env m (fn_params f ++ fn_vars f)) as [e m1] eqn:?.
-  myinv. left; right; apply step_internal_function with m1. auto.
-  change e with (fst (e,m1)). change m1 with (snd (e,m1)) at 2. rewrite <- Heqp.
-  apply do_alloc_variables_sound. eapply sem_bind_parameters_sound; eauto.
+  destruct p.
+  myinv. left; right.
+  exploit alloc_variables_record_spec; eauto.
+  intros (lnr & m2 & fa & AV & fablocks & fasize & RSB).
+  eapply step_internal_function. auto. eauto. eauto. rewrite fasize. rewrite Z.max_r. auto. apply Z.le_max_l. eauto. 
+  eapply sem_bind_parameters_sound; eauto.
   (* external *)
   destruct p as [[[w' tr] v] m']. myinv. left; right; constructor.
   eapply do_ef_external_sound; eauto.
@@ -2108,7 +2370,7 @@ Proof with try (left; right; econstructor; eauto; fail).
 Qed.
 
 Remark estep_not_val:
-  forall f a k e m t S, estep ge (ExprState f a k e m) t S -> is_val a = None.
+  forall f a k e m t S, estep ((*SACC:*)fn_stack_requirements) ge (ExprState f a k e m) t S -> is_val a = None.
 Proof.
   intros.
   assert (forall b from to C, context from to C -> (from = to /\ C = fun x => x) \/ is_val (C b) = None).
@@ -2120,9 +2382,53 @@ Proof.
   destruct (H0 a0 _ _ _ H8) as [[A B] | A]. subst. destruct a0; auto. elim H9. constructor. auto.
 Qed.
 
+(*SACC:*)
+Lemma frame_adt_eq:
+  forall fa1 fa2,
+    frame_adt_blocks fa1 = frame_adt_blocks fa2 ->
+    frame_adt_size fa1 = frame_adt_size fa2 ->
+    fa1 = fa2.
+Proof.
+  destruct fa1, fa2. simpl. intros A B.
+  subst. f_equal; apply proof_irr.
+Qed.
+
+(*SACC:*)
+Lemma constr_let:
+  forall {A1 A2 B: Type} (a: A1 * A2)
+    m b (EQ: a = (m,b))
+    (T: forall m b (pf: (m,b) = a), option B)
+    X
+    (EQ: T _ _ (eq_sym EQ) = Some X),
+    (let (m0,b0) as ano return (ano = a -> option B) := a in
+     fun Heq : (m0,b0) = a => T m0 b0 Heq) eq_refl = Some X.
+Proof.
+  intros. subst. simpl in *.  auto. 
+Qed.
+
+(*SACC:*)
+Lemma alloc_variables_record_complete:
+  forall f m e m1 fa m1',
+    list_norepet (var_names (fn_params f) ++ var_names (fn_vars f)) ->
+    alloc_variables ge empty_env m (fn_params f ++ fn_vars f) e m1 ->
+    frame_adt_blocks fa = blocks_with_info ge e ->
+    Mem.record_stack_blocks m1 fa = Some m1' ->
+    alloc_variables_record f m (frame_adt_size fa) = Some (e,m1').
+Proof.
+  intros.
+  unfold alloc_variables_record.
+  destr.
+  Focus 2. exfalso; apply n; auto.
+  eapply constr_let.
+  erewrite (frame_adt_eq fa) in H2.
+  rewrite H2. eauto. rewrite H1; reflexivity. simpl. rewrite Z.max_r; auto. destruct fa; auto.
+  Unshelve.
+  eapply do_alloc_variables_complete. eauto.
+Qed.
+
 Theorem do_step_complete:
   forall w S t S' w',
-  possible_trace w t w' -> Csem.step ge S t S' -> exists rule, In (TR rule t S') (do_step w S).
+  possible_trace w t w' -> Csem.step ((*SACC:*)fn_stack_requirements) ge S t S' -> exists rule, In (TR rule t S') (do_step w S).
 Proof with (unfold ret; eauto with coqlib).
   intros until w'; intros PT H.
   destruct H.
@@ -2151,7 +2457,8 @@ Proof with (unfold ret; eauto with coqlib).
   unfold do_step; rewrite NOTVAL.
   exploit callred_topred; eauto. instantiate (1 := w). instantiate (1 := e).
   intros (rule & STEP). exists rule.
-  change (TR rule E0 (Callstate fd vargs (Kcall f e C ty k) m)) with (expr_final_state f k e (C, Callred rule fd vargs ty m)).
+  change (TR rule E0 (Callstate fd vargs (Kcall f e C ty k) (Mem.push_new_stage m) (fn_stack_requirements fid))) 
+    with (expr_final_state f k e (C, Callred rule fd vargs ty (Mem.push_new_stage m) fid)).
   apply in_map.
   generalize (step_expr_context e w _ _ _ H1 a m). unfold reducts_incl.
   intro. replace C with (fun x => C x). apply H2.
@@ -2186,14 +2493,20 @@ Proof with (unfold ret; eauto with coqlib).
   rewrite H0...
 
   (* Call step *)
-  rewrite pred_dec_true; auto. rewrite (do_alloc_variables_complete _ _ _ _ _ H1).
-  rewrite (sem_bind_parameters_complete _ _ _ _ _ _ H2)...
+  rewrite <- H3. erewrite alloc_variables_record_complete; eauto.
+  rewrite (sem_bind_parameters_complete _ _ _ _ _ _ H5)...
   exploit do_ef_external_complete; eauto. intro EQ; rewrite EQ. auto with coqlib.
+
+  rewrite H0...
 Qed.
 
 End EXEC.
 
 Local Open Scope option_monad_scope.
+
+Section STACK_WRAPPER.
+
+Variable fn_stack_requirements: ident -> Z.
 
 Definition do_initial_state (p: program): option (genv * state) :=
   let ge := globalenv p in
@@ -2201,10 +2514,12 @@ Definition do_initial_state (p: program): option (genv * state) :=
   do b <- Genv.find_symbol ge p.(prog_main);
   do f <- Genv.find_funct_ptr ge b;
   check (type_eq (type_of_fundef f) (Tfunction Tnil type_int32s cc_default));
-  Some (ge, Callstate f nil Kstop m0).
+  Some (ge, Callstate f nil Kstop (Mem.push_new_stage m0) (fn_stack_requirements (prog_main p))).
 
 Definition at_final_state (S: state): option int :=
   match S with
   | Returnstate (Vint r) Kstop m => Some r
   | _ => None
   end.
+
+End STACK_WRAPPER.
